monadic cvc5 environment (#22)
* chore: find mindboggling problems

* chore: new monadic api

* fix: add missing cpp-level back

* chore: cleanup and doc before PR

* chore: remove non-monadic convenience term constructors

* chore: move instance sanity checks to tests

* chore: remove obsolete bindings

* chore: put cvc5 functions in `Env` namespace

* chore: bump to nightly, remove obsolete code

* chore: expose term manager, wrap its functions in (Base)IO

* chore: format `ffi/ffi.cpp`

* chore: merge

* fix: use correct C++ signature for term manager constructor

* chore: make constructor names more consistent

ffi/ffi.cpp
@@ -13,7 +13,12 @@ lean_obj_res prod_mk(lean_obj_arg T,
 
 // ## `Except Error α` constructors
 
-lean_obj_res except_ok(lean_obj_arg alpha, lean_obj_arg val);
+lean_obj_res generic_except_ok(lean_obj_arg alpha, lean_obj_arg val);
+
+lean_obj_res except_ok(lean_obj_arg val)
+{
+  return generic_except_ok(lean_box(0), val);
+}
 
 lean_obj_res except_ok_bool(uint8_t val);
 
@@ -46,57 +51,50 @@ lean_obj_res except_err(lean_obj_arg alpha, lean_obj_arg msg);
         lean_mk_string("cvc5's term manager raised an unexpected exception")); \
   }
 
-// ## `SolverT` constructors
+// ## `Env` constructors
 
-lean_obj_res solver_val(lean_obj_arg m,
-                        lean_obj_arg inst,
-                        lean_obj_arg alpha,
-                        lean_obj_arg a,
-                        lean_obj_arg solver);
+lean_obj_res env_pure(lean_obj_arg alpha, lean_obj_arg a, lean_obj_arg ioWorld);
 
-lean_obj_res solver_err(lean_obj_arg m,
-                        lean_obj_arg inst,
-                        lean_obj_arg alpha,
-                        lean_obj_arg e,
-                        lean_obj_arg solver);
+lean_obj_res env_val(lean_obj_arg val, lean_obj_arg ioWorld)
+{
+  return env_pure(lean_box(0), val, ioWorld);
+}
 
-lean_obj_res solver_errOfString(lean_obj_arg m,
-                                lean_obj_arg inst,
-                                lean_obj_arg alpha,
-                                lean_obj_arg msg,
-                                lean_obj_arg solver);
+lean_obj_res env_throw(lean_obj_arg alpha,
+                       lean_obj_arg e,
+                       lean_obj_arg ioWorld);
 
-// ## Exception-catching macro for `SolverT`
-//
-// Runs `code`, `return`s an `Error` for `SolverT` on exceptions.
-//
-// - `inst`: monad instance.
-// - `solver`: solver state value.
-// - `code`: the code to run and catch exceptions for.
+lean_obj_res env_error(lean_obj_arg e, lean_obj_arg ioWorld)
+{
+  return env_throw(lean_box(0), e, ioWorld);
+}
 
-#define CVC5_LEAN_API_TRY_CATCH_SOLVER_BEGIN \
-  try                                        \
+lean_obj_res env_throw_string(lean_obj_arg alpha,
+                              lean_obj_arg msg,
+                              lean_obj_arg ioWorld);
+
+lean_obj_res env_error_string(lean_obj_arg e, lean_obj_arg ioWorld)
+{
+  return env_throw_string(lean_box(0), e, ioWorld);
+}
+
+#define CVC5_LEAN_API_TRY_CATCH_ENV_BEGIN \
+  try                                     \
   {
-#define CVC5_LEAN_API_TRY_CATCH_SOLVER_END(inst, solver)                   \
-  }                                                                        \
-  catch (CVC5ApiException & e)                                             \
-  {                                                                        \
-    return solver_errOfString(                                             \
-        lean_box(0), inst, lean_box(0), lean_mk_string(e.what()), solver); \
-  }                                                                        \
-  catch (char const* e)                                                    \
-  {                                                                        \
-    return solver_errOfString(                                             \
-        lean_box(0), inst, lean_box(0), lean_mk_string(e), solver);        \
-  }                                                                        \
-  catch (...)                                                              \
-  {                                                                        \
-    return solver_errOfString(                                             \
-        lean_box(0),                                                       \
-        inst,                                                              \
-        lean_box(0),                                                       \
-        lean_mk_string("cvc5 raised an unexpected exception"),             \
-        solver);                                                           \
+#define CVC5_LEAN_API_TRY_CATCH_ENV_END(ioWorld)                         \
+  }                                                                      \
+  catch (CVC5ApiException & e)                                           \
+  {                                                                      \
+    return env_error_string(lean_mk_string(e.what()), ioWorld);          \
+  }                                                                      \
+  catch (char const* e)                                                  \
+  {                                                                      \
+    return env_error_string(lean_mk_string(e), ioWorld);                 \
+  }                                                                      \
+  catch (...)                                                            \
+  {                                                                      \
+    return env_error_string(                                             \
+        lean_mk_string("cvc5 raised an unexpected exception"), ioWorld); \
   }
 
 inline lean_obj_res mk_unit_unit() { return lean_box(0); }
@@ -518,8 +516,7 @@ LEAN_EXPORT uint64_t sort_hash(lean_obj_arg s)
 LEAN_EXPORT lean_obj_res sort_getFunctionArity(lean_obj_arg s)
 {
   CVC5_LEAN_API_TRY_CATCH_EXCEPT_BEGIN;
-  return except_ok(lean_box(0),
-                   lean_usize_to_nat(sort_unbox(s)->getFunctionArity()));
+  return except_ok(lean_usize_to_nat(sort_unbox(s)->getFunctionArity()));
   CVC5_LEAN_API_TRY_CATCH_EXCEPT_END;
 }
 
@@ -532,7 +529,7 @@ LEAN_EXPORT lean_obj_res sort_getFunctionDomainSorts(lean_obj_arg s)
   {
     ds = lean_array_push(ds, sort_box(new Sort(domain)));
   }
-  return except_ok(lean_box(0), ds);
+  return except_ok(ds);
   CVC5_LEAN_API_TRY_CATCH_EXCEPT_END;
 }
 
@@ -540,7 +537,6 @@ LEAN_EXPORT lean_obj_res sort_getFunctionCodomainSort(lean_obj_arg s)
 {
   CVC5_LEAN_API_TRY_CATCH_EXCEPT_BEGIN;
   return except_ok(
-      lean_box(0),
       sort_box(new Sort(sort_unbox(s)->getFunctionCodomainSort())));
   CVC5_LEAN_API_TRY_CATCH_EXCEPT_END;
 }
@@ -548,40 +544,35 @@ LEAN_EXPORT lean_obj_res sort_getFunctionCodomainSort(lean_obj_arg s)
 LEAN_EXPORT lean_obj_res sort_getArrayIndexSort(lean_obj_arg s)
 {
   CVC5_LEAN_API_TRY_CATCH_EXCEPT_BEGIN;
-  return except_ok(lean_box(0),
-                   sort_box(new Sort(sort_unbox(s)->getArrayIndexSort())));
+  return except_ok(sort_box(new Sort(sort_unbox(s)->getArrayIndexSort())));
   CVC5_LEAN_API_TRY_CATCH_EXCEPT_END;
 }
 
 LEAN_EXPORT lean_obj_res sort_getArrayElementSort(lean_obj_arg s)
 {
   CVC5_LEAN_API_TRY_CATCH_EXCEPT_BEGIN;
-  return except_ok(lean_box(0),
-                   sort_box(new Sort(sort_unbox(s)->getArrayElementSort())));
+  return except_ok(sort_box(new Sort(sort_unbox(s)->getArrayElementSort())));
   CVC5_LEAN_API_TRY_CATCH_EXCEPT_END;
 }
 
 LEAN_EXPORT lean_obj_res sort_getSetElementSort(lean_obj_arg s)
 {
   CVC5_LEAN_API_TRY_CATCH_EXCEPT_BEGIN;
-  return except_ok(lean_box(0),
-                   sort_box(new Sort(sort_unbox(s)->getSetElementSort())));
+  return except_ok(sort_box(new Sort(sort_unbox(s)->getSetElementSort())));
   CVC5_LEAN_API_TRY_CATCH_EXCEPT_END;
 }
 
 LEAN_EXPORT lean_obj_res sort_getBagElementSort(lean_obj_arg s)
 {
   CVC5_LEAN_API_TRY_CATCH_EXCEPT_BEGIN;
-  return except_ok(lean_box(0),
-                   sort_box(new Sort(sort_unbox(s)->getBagElementSort())));
+  return except_ok(sort_box(new Sort(sort_unbox(s)->getBagElementSort())));
   CVC5_LEAN_API_TRY_CATCH_EXCEPT_END;
 }
 
 LEAN_EXPORT lean_obj_res sort_getSequenceElementSort(lean_obj_arg s)
 {
   CVC5_LEAN_API_TRY_CATCH_EXCEPT_BEGIN;
-  return except_ok(lean_box(0),
-                   sort_box(new Sort(sort_unbox(s)->getSequenceElementSort())));
+  return except_ok(sort_box(new Sort(sort_unbox(s)->getSequenceElementSort())));
   CVC5_LEAN_API_TRY_CATCH_EXCEPT_END;
 }
 
@@ -603,8 +594,7 @@ LEAN_EXPORT lean_obj_res sort_hasSymbol(lean_obj_arg s)
 LEAN_EXPORT lean_obj_res sort_getSymbol(lean_obj_arg s)
 {
   CVC5_LEAN_API_TRY_CATCH_EXCEPT_BEGIN;
-  return except_ok(lean_box(0),
-                   lean_mk_string(sort_unbox(s)->getSymbol().c_str()));
+  return except_ok(lean_mk_string(sort_unbox(s)->getSymbol().c_str()));
   CVC5_LEAN_API_TRY_CATCH_EXCEPT_END;
 }
 
@@ -628,7 +618,6 @@ LEAN_EXPORT lean_obj_res sort_getFiniteFieldSize(lean_obj_arg s)
 {
   CVC5_LEAN_API_TRY_CATCH_EXCEPT_BEGIN;
   return except_ok(
-      lean_box(0),
       lean_cstr_to_nat(sort_unbox(s)->getFiniteFieldSize().c_str()));
   CVC5_LEAN_API_TRY_CATCH_EXCEPT_END;
 }
@@ -658,22 +647,21 @@ LEAN_EXPORT lean_obj_res sort_getTupleLength(lean_obj_arg s)
 
 LEAN_EXPORT lean_obj_res sort_getTupleSorts(lean_obj_arg s)
 {
-  CVC5_LEAN_API_TRY_CATCH_SOLVER_BEGIN;
+  CVC5_LEAN_API_TRY_CATCH_EXCEPT_BEGIN;
   std::vector<Sort> sorts = sort_unbox(s)->getTupleSorts();
   lean_object* array = lean_mk_empty_array();
   for (const Sort& sort : sorts)
   {
     array = lean_array_push(array, sort_box(new Sort(sort)));
   }
-  return except_ok(lean_box(0), array);
+  return except_ok(array);
   CVC5_LEAN_API_TRY_CATCH_EXCEPT_END;
 }
 
 LEAN_EXPORT lean_obj_res sort_getNullableElementSort(lean_obj_arg s)
 {
   CVC5_LEAN_API_TRY_CATCH_EXCEPT_BEGIN;
-  return except_ok(lean_box(0),
-                   sort_box(new Sort(sort_unbox(s)->getNullableElementSort())));
+  return except_ok(sort_box(new Sort(sort_unbox(s)->getNullableElementSort())));
   CVC5_LEAN_API_TRY_CATCH_EXCEPT_END;
 }
 
@@ -681,7 +669,6 @@ LEAN_EXPORT lean_obj_res sort_getUninterpretedSortConstructor(lean_obj_arg s)
 {
   CVC5_LEAN_API_TRY_CATCH_EXCEPT_BEGIN;
   return except_ok(
-      lean_box(0),
       sort_box(new Sort((sort_unbox(s)->getUninterpretedSortConstructor()))));
   CVC5_LEAN_API_TRY_CATCH_EXCEPT_END;
 }
@@ -695,7 +682,7 @@ LEAN_EXPORT lean_obj_res sort_getInstantiatedParameters(lean_obj_arg s)
   {
     ps = lean_array_push(ps, sort_box(new Sort(param)));
   }
-  return except_ok(lean_box(0), ps);
+  return except_ok(ps);
   CVC5_LEAN_API_TRY_CATCH_EXCEPT_END;
 }
 
@@ -708,8 +695,7 @@ LEAN_EXPORT lean_obj_arg sort_instantiate(lean_obj_arg s, lean_obj_arg params)
     cvc5Sorts.push_back(*sort_unbox(
         lean_array_get(sort_box(new Sort()), params, lean_usize_to_nat(i))));
   }
-  return except_ok(lean_box(0),
-                   sort_box(new Sort(sort_unbox(s)->instantiate(cvc5Sorts))));
+  return except_ok(sort_box(new Sort(sort_unbox(s)->instantiate(cvc5Sorts))));
   CVC5_LEAN_API_TRY_CATCH_EXCEPT_END;
 }
 
@@ -730,9 +716,8 @@ LEAN_EXPORT lean_obj_arg sort_substitute(lean_obj_arg s,
     cvc5Replacements.push_back(*sort_unbox(lean_array_get(
         sort_box(new Sort()), replacements, lean_usize_to_nat(i))));
   }
-  return except_ok(lean_box(0),
-                   sort_box(new Sort(sort_unbox(s)->substitute(
-                       cvc5Sorts, cvc5Replacements))));
+  return except_ok(sort_box(
+      new Sort(sort_unbox(s)->substitute(cvc5Sorts, cvc5Replacements))));
   CVC5_LEAN_API_TRY_CATCH_EXCEPT_END;
 }
 
@@ -844,7 +829,7 @@ LEAN_EXPORT uint8_t term_isNull(lean_obj_arg t)
 LEAN_EXPORT lean_obj_res term_not(lean_obj_arg t)
 {
   CVC5_LEAN_API_TRY_CATCH_EXCEPT_BEGIN;
-  return except_ok(lean_box(0), term_box(new Term(term_unbox(t)->notTerm())));
+  return except_ok(term_box(new Term(term_unbox(t)->notTerm())));
   CVC5_LEAN_API_TRY_CATCH_EXCEPT_END;
 }
 
@@ -852,7 +837,6 @@ LEAN_EXPORT lean_obj_res term_and(lean_obj_arg t1, lean_obj_arg t2)
 {
   CVC5_LEAN_API_TRY_CATCH_EXCEPT_BEGIN;
   return except_ok(
-      lean_box(0),
       term_box(new Term(term_unbox(t1)->andTerm(*term_unbox(t2)))));
   CVC5_LEAN_API_TRY_CATCH_EXCEPT_END;
 }
@@ -860,8 +844,7 @@ LEAN_EXPORT lean_obj_res term_and(lean_obj_arg t1, lean_obj_arg t2)
 LEAN_EXPORT lean_obj_res term_or(lean_obj_arg t1, lean_obj_arg t2)
 {
   CVC5_LEAN_API_TRY_CATCH_EXCEPT_BEGIN;
-  return except_ok(lean_box(0),
-                   term_box(new Term(term_unbox(t1)->orTerm(*term_unbox(t2)))));
+  return except_ok(term_box(new Term(term_unbox(t1)->orTerm(*term_unbox(t2)))));
   CVC5_LEAN_API_TRY_CATCH_EXCEPT_END;
 }
 
@@ -869,7 +852,6 @@ LEAN_EXPORT lean_obj_res term_xor(lean_obj_arg t1, lean_obj_arg t2)
 {
   CVC5_LEAN_API_TRY_CATCH_EXCEPT_BEGIN;
   return except_ok(
-      lean_box(0),
       term_box(new Term(term_unbox(t1)->xorTerm(*term_unbox(t2)))));
   CVC5_LEAN_API_TRY_CATCH_EXCEPT_END;
 }
@@ -877,8 +859,7 @@ LEAN_EXPORT lean_obj_res term_xor(lean_obj_arg t1, lean_obj_arg t2)
 LEAN_EXPORT lean_obj_res term_eq(lean_obj_arg t1, lean_obj_arg t2)
 {
   CVC5_LEAN_API_TRY_CATCH_EXCEPT_BEGIN;
-  return except_ok(lean_box(0),
-                   term_box(new Term(term_unbox(t1)->eqTerm(*term_unbox(t2)))));
+  return except_ok(term_box(new Term(term_unbox(t1)->eqTerm(*term_unbox(t2)))));
   CVC5_LEAN_API_TRY_CATCH_EXCEPT_END;
 }
 
@@ -886,7 +867,6 @@ LEAN_EXPORT lean_obj_res term_imp(lean_obj_arg t1, lean_obj_arg t2)
 {
   CVC5_LEAN_API_TRY_CATCH_EXCEPT_BEGIN;
   return except_ok(
-      lean_box(0),
       term_box(new Term(term_unbox(t1)->impTerm(*term_unbox(t2)))));
   CVC5_LEAN_API_TRY_CATCH_EXCEPT_END;
 }
@@ -896,9 +876,8 @@ LEAN_EXPORT lean_obj_res term_ite(lean_obj_arg t1,
                                   lean_obj_arg t3)
 {
   CVC5_LEAN_API_TRY_CATCH_EXCEPT_BEGIN;
-  return except_ok(lean_box(0),
-                   term_box(new Term(term_unbox(t1)->iteTerm(
-                       *term_unbox(t2), *term_unbox(t3)))));
+  return except_ok(term_box(
+      new Term(term_unbox(t1)->iteTerm(*term_unbox(t2), *term_unbox(t3)))));
   CVC5_LEAN_API_TRY_CATCH_EXCEPT_END;
 }
 
@@ -920,7 +899,7 @@ LEAN_EXPORT uint8_t term_hasOp(lean_obj_arg t)
 LEAN_EXPORT lean_obj_arg term_getOp(lean_obj_arg t)
 {
   CVC5_LEAN_API_TRY_CATCH_EXCEPT_BEGIN;
-  return except_ok(lean_box(0), op_box(new Op(term_unbox(t)->getOp())));
+  return except_ok(op_box(new Op(term_unbox(t)->getOp())));
   CVC5_LEAN_API_TRY_CATCH_EXCEPT_END;
 }
 
@@ -950,7 +929,6 @@ LEAN_EXPORT lean_obj_res term_getBitVectorValue(lean_obj_arg t, uint32_t base)
 {
   CVC5_LEAN_API_TRY_CATCH_EXCEPT_BEGIN;
   return except_ok(
-      lean_box(0),
       lean_mk_string(term_unbox(t)->getBitVectorValue(base).c_str()));
   CVC5_LEAN_API_TRY_CATCH_EXCEPT_END;
 }
@@ -958,8 +936,7 @@ LEAN_EXPORT lean_obj_res term_getBitVectorValue(lean_obj_arg t, uint32_t base)
 LEAN_EXPORT lean_obj_res term_getIntegerValue(lean_obj_arg t)
 {
   CVC5_LEAN_API_TRY_CATCH_EXCEPT_BEGIN;
-  return except_ok(lean_box(0),
-                   lean_cstr_to_int(term_unbox(t)->getIntegerValue().c_str()));
+  return except_ok(lean_cstr_to_int(term_unbox(t)->getIntegerValue().c_str()));
   CVC5_LEAN_API_TRY_CATCH_EXCEPT_END;
 }
 
@@ -972,7 +949,6 @@ LEAN_EXPORT lean_obj_res term_getRationalValue(lean_obj_arg t)
   std::string r = term_unbox(t)->getRealValue();
   size_t i = r.find('/');
   return except_ok(
-      lean_box(0),
       l_Std_Internal_mkRat(lean_cstr_to_int(r.substr(0, i).c_str()),
                            lean_cstr_to_nat(r.substr(i + 1).c_str())));
   CVC5_LEAN_API_TRY_CATCH_EXCEPT_END;
@@ -986,8 +962,7 @@ LEAN_EXPORT uint8_t term_hasSymbol(lean_obj_arg t)
 LEAN_EXPORT lean_obj_res term_getSymbol(lean_obj_arg t)
 {
   CVC5_LEAN_API_TRY_CATCH_EXCEPT_BEGIN;
-  return except_ok(lean_box(0),
-                   lean_mk_string(term_unbox(t)->getSymbol().c_str()));
+  return except_ok(lean_mk_string(term_unbox(t)->getSymbol().c_str()));
   CVC5_LEAN_API_TRY_CATCH_EXCEPT_END;
 }
 
@@ -1022,7 +997,7 @@ LEAN_EXPORT lean_obj_res term_getSkolemIndices(lean_obj_arg t)
   {
     as = lean_array_push(as, term_box(new Term(arg)));
   }
-  return except_ok(lean_box(0), as);
+  return except_ok(as);
   CVC5_LEAN_API_TRY_CATCH_EXCEPT_END;
 }
 
@@ -1140,302 +1115,11 @@ static inline TermManager* mut_tm_unbox(b_lean_obj_arg tm)
   return static_cast<TermManager*>(lean_get_external_data(tm));
 }
 
-LEAN_EXPORT lean_obj_res termManager_new(lean_obj_arg unit)
+LEAN_EXPORT lean_obj_res termManager_new(lean_obj_arg ioWorld)
 {
-  return lean_io_result_mk_ok(tm_box(new TermManager()));
-}
-
-LEAN_EXPORT lean_obj_arg termManager_getBooleanSort(lean_obj_arg tm)
-{
-  return sort_box(new Sort(mut_tm_unbox(tm)->getBooleanSort()));
-}
-
-LEAN_EXPORT lean_obj_arg termManager_getIntegerSort(lean_obj_arg tm)
-{
-  return sort_box(new Sort(mut_tm_unbox(tm)->getIntegerSort()));
-}
-
-LEAN_EXPORT lean_obj_arg termManager_getRealSort(lean_obj_arg tm)
-{
-  return sort_box(new Sort(mut_tm_unbox(tm)->getRealSort()));
-}
-
-LEAN_EXPORT lean_obj_arg termManager_getRegExpSort(lean_obj_arg tm)
-{
-  return sort_box(new Sort(mut_tm_unbox(tm)->getRegExpSort()));
-}
-
-LEAN_EXPORT lean_obj_arg termManager_getRoundingModeSort(lean_obj_arg tm)
-{
-  return sort_box(new Sort(mut_tm_unbox(tm)->getRoundingModeSort()));
-}
-
-LEAN_EXPORT lean_obj_arg termManager_getStringSort(lean_obj_arg tm)
-{
-  return sort_box(new Sort(mut_tm_unbox(tm)->getStringSort()));
-}
-
-LEAN_EXPORT lean_obj_arg termManager_mkArraySort(lean_obj_arg tm,
-                                                 lean_obj_arg idx,
-                                                 lean_obj_arg elm)
-{
-  CVC5_LEAN_API_TRY_CATCH_EXCEPT_BEGIN;
-  return except_ok(lean_box(0),
-                   sort_box(new Sort(mut_tm_unbox(tm)->mkArraySort(
-                       *sort_unbox(idx), *sort_unbox(elm)))));
-  CVC5_LEAN_API_TRY_CATCH_EXCEPT_END;
-}
-
-LEAN_EXPORT lean_obj_arg termManager_mkBitVectorSort(lean_obj_arg tm,
-                                                     uint32_t size)
-{
-  CVC5_LEAN_API_TRY_CATCH_EXCEPT_BEGIN;
-  return except_ok(lean_box(0),
-                   sort_box(new Sort(mut_tm_unbox(tm)->mkBitVectorSort(size))));
-  CVC5_LEAN_API_TRY_CATCH_EXCEPT_END;
-}
-
-LEAN_EXPORT lean_obj_arg termManager_mkFloatingPointSort(lean_obj_arg tm,
-                                                         uint32_t exp,
-                                                         uint32_t sig)
-{
-  CVC5_LEAN_API_TRY_CATCH_EXCEPT_BEGIN;
-  return except_ok(
-      lean_box(0),
-      sort_box(new Sort(mut_tm_unbox(tm)->mkFloatingPointSort(exp, sig))));
-  CVC5_LEAN_API_TRY_CATCH_EXCEPT_END;
-}
-
-LEAN_EXPORT lean_obj_arg termManager_mkFiniteFieldSortFromString(
-    lean_obj_arg tm, lean_obj_arg size, uint32_t base)
-{
-  CVC5_LEAN_API_TRY_CATCH_EXCEPT_BEGIN;
-  return except_ok(lean_box(0),
-                   sort_box(new Sort(mut_tm_unbox(tm)->mkFiniteFieldSort(
-                       lean_string_cstr(size), base))));
-  CVC5_LEAN_API_TRY_CATCH_EXCEPT_END;
-}
-
-LEAN_EXPORT lean_obj_arg termManager_mkFunctionSort(lean_obj_arg tm,
-                                                    lean_obj_arg sorts,
-                                                    lean_obj_arg codomain)
-{
-  CVC5_LEAN_API_TRY_CATCH_EXCEPT_BEGIN;
-  std::vector<Sort> cvc5Sorts;
-  for (size_t i = 0, n = lean_array_size(sorts); i < n; ++i)
-  {
-    cvc5Sorts.push_back(*sort_unbox(
-        lean_array_get(sort_box(new Sort()), sorts, lean_usize_to_nat(i))));
-  }
-  return except_ok(lean_box(0),
-                   sort_box(new Sort(mut_tm_unbox(tm)->mkFunctionSort(
-                       cvc5Sorts, *sort_unbox(codomain)))));
-  CVC5_LEAN_API_TRY_CATCH_EXCEPT_END;
-}
-
-LEAN_EXPORT lean_obj_arg termManager_mkPredicateSort(lean_obj_arg tm,
-                                                     lean_obj_arg sorts)
-{
-  CVC5_LEAN_API_TRY_CATCH_EXCEPT_BEGIN;
-  std::vector<Sort> cvc5Sorts;
-  for (size_t i = 0, n = lean_array_size(sorts); i < n; ++i)
-  {
-    cvc5Sorts.push_back(*sort_unbox(
-        lean_array_get(sort_box(new Sort()), sorts, lean_usize_to_nat(i))));
-  }
-  return except_ok(
-      lean_box(0),
-      sort_box(new Sort(mut_tm_unbox(tm)->mkPredicateSort(cvc5Sorts))));
-  CVC5_LEAN_API_TRY_CATCH_EXCEPT_END;
-}
-
-LEAN_EXPORT lean_obj_res termManager_mkSetSort(lean_obj_arg tm,
-                                               lean_obj_arg sort)
-{
-  CVC5_LEAN_API_TRY_CATCH_EXCEPT_BEGIN;
-  return except_ok(
-      lean_box(0),
-      sort_box(new Sort(mut_tm_unbox(tm)->mkSetSort(*sort_unbox(sort)))));
-  CVC5_LEAN_API_TRY_CATCH_EXCEPT_END;
-}
-
-LEAN_EXPORT lean_obj_res termManager_mkBagSort(lean_obj_arg tm,
-                                               lean_obj_arg sort)
-{
-  CVC5_LEAN_API_TRY_CATCH_EXCEPT_BEGIN;
-  return except_ok(
-      lean_box(0),
-      sort_box(new Sort(mut_tm_unbox(tm)->mkBagSort(*sort_unbox(sort)))));
-  CVC5_LEAN_API_TRY_CATCH_EXCEPT_END;
-}
-
-LEAN_EXPORT lean_obj_res termManager_mkSequenceSort(lean_obj_arg tm,
-                                                    lean_obj_arg sort)
-{
-  CVC5_LEAN_API_TRY_CATCH_EXCEPT_BEGIN;
-  return except_ok(
-      lean_box(0),
-      sort_box(new Sort(mut_tm_unbox(tm)->mkSequenceSort(*sort_unbox(sort)))));
-  CVC5_LEAN_API_TRY_CATCH_EXCEPT_END;
-}
-
-LEAN_EXPORT lean_obj_res termManager_mkAbstractSort(lean_obj_arg tm,
-                                                    uint16_t kind)
-{
-  CVC5_LEAN_API_TRY_CATCH_EXCEPT_BEGIN;
-  SortKind k = static_cast<SortKind>(static_cast<int32_t>(kind) - 2);
-  return except_ok(lean_box(0),
-                   sort_box(new Sort(mut_tm_unbox(tm)->mkAbstractSort(k))));
-  CVC5_LEAN_API_TRY_CATCH_EXCEPT_END;
-}
-
-LEAN_EXPORT lean_obj_res termManager_mkUninterpretedSort(lean_obj_arg tm,
-                                                         lean_obj_arg symbol)
-{
-  return sort_box(new Sort(
-      mut_tm_unbox(tm)->mkUninterpretedSort(lean_string_cstr(symbol))));
-}
-
-LEAN_EXPORT lean_obj_arg termManager_mkUninterpretedSortConstructorSort(
-    lean_obj_arg tm, lean_obj_arg arity, lean_obj_arg symbol)
-{
-  CVC5_LEAN_API_TRY_CATCH_EXCEPT_BEGIN;
-  return except_ok(
-      lean_box(0),
-      sort_box(new Sort(mut_tm_unbox(tm)->mkUninterpretedSortConstructorSort(
-          lean_usize_of_nat(arity), lean_string_cstr(symbol)))));
-  CVC5_LEAN_API_TRY_CATCH_EXCEPT_END;
-}
-
-LEAN_EXPORT lean_obj_arg termManager_mkTupleSort(lean_obj_arg tm,
-                                                 lean_obj_arg sorts)
-{
-  CVC5_LEAN_API_TRY_CATCH_EXCEPT_BEGIN;
-  std::vector<Sort> cvc5Sorts;
-  for (size_t i = 0, n = lean_array_size(sorts); i < n; ++i)
-  {
-    cvc5Sorts.push_back(*sort_unbox(
-        lean_array_get(sort_box(new Sort()), sorts, lean_usize_to_nat(i))));
-  }
-  return except_ok(
-      lean_box(0),
-      sort_box(new Sort(mut_tm_unbox(tm)->mkTupleSort(cvc5Sorts))));
-  CVC5_LEAN_API_TRY_CATCH_EXCEPT_END;
-}
-
-LEAN_EXPORT lean_obj_res termManager_mkNullableSort(lean_obj_arg tm,
-                                                    lean_obj_arg sort)
-{
-  CVC5_LEAN_API_TRY_CATCH_EXCEPT_BEGIN;
-  return except_ok(
-      lean_box(0),
-      sort_box(new Sort(mut_tm_unbox(tm)->mkNullableSort(*sort_unbox(sort)))));
-  CVC5_LEAN_API_TRY_CATCH_EXCEPT_END;
-}
-
-LEAN_EXPORT lean_obj_res termManager_mkParamSort(lean_obj_arg tm,
-                                                 lean_obj_arg symbol)
-{
-  return sort_box(
-      new Sort(mut_tm_unbox(tm)->mkParamSort(lean_string_cstr(symbol))));
-}
-
-LEAN_EXPORT lean_obj_res termManager_mkBoolean(lean_obj_arg tm, uint8_t val)
-{
-  return term_box(new Term(mut_tm_unbox(tm)->mkBoolean(bool_unbox(val))));
-}
-
-LEAN_EXPORT lean_obj_res termManager_mkIntegerFromString(lean_obj_arg tm,
-                                                         lean_obj_arg val)
-{
-  CVC5_LEAN_API_TRY_CATCH_EXCEPT_BEGIN;
-  return except_ok(
-      lean_box(0),
-      term_box(new Term(mut_tm_unbox(tm)->mkInteger(lean_string_cstr(val)))));
-  CVC5_LEAN_API_TRY_CATCH_EXCEPT_END;
-}
-
-LEAN_EXPORT lean_obj_res termManager_mkRealFromString(lean_obj_arg tm,
-                                                      lean_obj_arg val)
-{
-  CVC5_LEAN_API_TRY_CATCH_EXCEPT_BEGIN;
-  return except_ok(
-      lean_box(0),
-      term_box(new Term(mut_tm_unbox(tm)->mkReal(lean_string_cstr(val)))));
-  CVC5_LEAN_API_TRY_CATCH_EXCEPT_END;
-}
-
-LEAN_EXPORT lean_obj_res termManager_mkTerm(lean_obj_arg tm,
-                                            uint16_t kind,
-                                            lean_obj_arg children)
-{
-  CVC5_LEAN_API_TRY_CATCH_EXCEPT_BEGIN;
-  Kind k = static_cast<Kind>(static_cast<int32_t>(kind) - 2);
-  std::vector<Term> cs;
-  for (size_t i = 0, n = lean_array_size(children); i < n; ++i)
-  {
-    cs.push_back(*term_unbox(
-        lean_array_get(term_box(new Term()), children, lean_usize_to_nat(i))));
-  }
-  return except_ok(lean_box(0),
-                   term_box(new Term(mut_tm_unbox(tm)->mkTerm(k, cs))));
-  CVC5_LEAN_API_TRY_CATCH_EXCEPT_END;
-}
-
-LEAN_EXPORT lean_obj_res termManager_mkTermOfOp(lean_obj_arg tm,
-                                                lean_obj_arg op,
-                                                lean_obj_arg children)
-{
-  CVC5_LEAN_API_TRY_CATCH_EXCEPT_BEGIN;
-  std::vector<Term> cs;
-  for (size_t i = 0, n = lean_array_size(children); i < n; ++i)
-  {
-    cs.push_back(*term_unbox(
-        lean_array_get(term_box(new Term()), children, lean_usize_to_nat(i))));
-  }
-  return except_ok(
-      lean_box(0),
-      term_box(new Term(mut_tm_unbox(tm)->mkTerm(*op_unbox(op), cs))));
-  CVC5_LEAN_API_TRY_CATCH_EXCEPT_END;
-}
-
-// This function is not part of the *public* `lean-cvc5` API: it produces a
-// different (fresh) term every time it's called which is really bad for purity.
-LEAN_EXPORT lean_obj_res termManager_mkConst(lean_obj_arg tm,
-                                             lean_obj_arg sort,
-                                             lean_obj_arg symbol)
-{
-  return term_box(new Term(
-      mut_tm_unbox(tm)->mkConst(*sort_unbox(sort), lean_string_cstr(symbol))));
-}
-
-LEAN_EXPORT lean_obj_res termManager_mkOpOfIndices(lean_obj_arg tm,
-                                                   uint16_t kind,
-                                                   lean_obj_arg args)
-{
-  CVC5_LEAN_API_TRY_CATCH_EXCEPT_BEGIN;
-  Kind k = static_cast<Kind>(static_cast<int32_t>(kind) - 2);
-  std::vector<uint32_t> indices;
-  for (size_t i = 0, n = lean_array_size(args); i < n; ++i)
-  {
-    indices.push_back(lean_uint32_of_nat_mk(
-        lean_array_get(lean_usize_to_nat(0), args, lean_usize_to_nat(i))));
-  }
-  return except_ok(lean_box(0),
-                   op_box(new Op(mut_tm_unbox(tm)->mkOp(k, indices))));
-  CVC5_LEAN_API_TRY_CATCH_EXCEPT_END;
-}
-
-LEAN_EXPORT lean_obj_res termManager_mkOpOfString(lean_obj_arg tm,
-                                                  uint16_t kind,
-                                                  lean_obj_arg arg)
-{
-  CVC5_LEAN_API_TRY_CATCH_EXCEPT_BEGIN;
-  Kind k = static_cast<Kind>(static_cast<int32_t>(kind) - 2);
-  return except_ok(
-      lean_box(0),
-      op_box(new Op(mut_tm_unbox(tm)->mkOp(k, lean_string_cstr(arg)))));
-  CVC5_LEAN_API_TRY_CATCH_EXCEPT_END;
+  CVC5_LEAN_API_TRY_CATCH_ENV_BEGIN;
+  return env_val(tm_box(new TermManager()), ioWorld);
+  CVC5_LEAN_API_TRY_CATCH_ENV_END(ioWorld);
 }
 
 static void solver_finalize(void* obj) { delete static_cast<Solver*>(obj); }
@@ -1462,224 +1146,588 @@ static inline Solver* solver_unbox(b_lean_obj_arg s)
   return static_cast<Solver*>(lean_get_external_data(s));
 }
 
-LEAN_EXPORT lean_obj_res solver_new(lean_obj_arg tm)
+// # Sorts
+
+LEAN_EXPORT lean_obj_res termManager_getBooleanSort(lean_obj_arg tm,
+                                                    lean_obj_arg ioWorld)
 {
-  return solver_box(new Solver(*mut_tm_unbox(tm)));
+  CVC5_LEAN_API_TRY_CATCH_ENV_BEGIN;
+  return env_val(sort_box(new Sort(mut_tm_unbox(tm)->getBooleanSort())),
+                 ioWorld);
+  CVC5_LEAN_API_TRY_CATCH_ENV_END(ioWorld);
 }
 
-LEAN_EXPORT lean_obj_res solver_getVersion(lean_obj_arg inst,
-                                           lean_obj_arg solver)
+LEAN_EXPORT lean_obj_res termManager_getIntegerSort(lean_obj_arg tm,
+                                                    lean_obj_arg ioWorld)
 {
-  CVC5_LEAN_API_TRY_CATCH_SOLVER_BEGIN;
-  return solver_val(lean_box(0),
-                    inst,
-                    lean_box(0),
-                    lean_mk_string(solver_unbox(solver)->getVersion().c_str()),
-                    solver);
-  CVC5_LEAN_API_TRY_CATCH_SOLVER_END(inst, solver);
+  CVC5_LEAN_API_TRY_CATCH_ENV_BEGIN;
+  return env_val(sort_box(new Sort(mut_tm_unbox(tm)->getIntegerSort())),
+                 ioWorld);
+  CVC5_LEAN_API_TRY_CATCH_ENV_END(ioWorld);
 }
 
-LEAN_EXPORT lean_obj_res solver_setOption(lean_obj_arg inst,
+LEAN_EXPORT lean_obj_res termManager_getRealSort(lean_obj_arg tm,
+                                                 lean_obj_arg ioWorld)
+{
+  CVC5_LEAN_API_TRY_CATCH_ENV_BEGIN;
+  return env_val(sort_box(new Sort(mut_tm_unbox(tm)->getRealSort())), ioWorld);
+  CVC5_LEAN_API_TRY_CATCH_ENV_END(ioWorld);
+}
+
+LEAN_EXPORT lean_obj_res termManager_getRegExpSort(lean_obj_arg tm,
+                                                   lean_obj_arg ioWorld)
+{
+  CVC5_LEAN_API_TRY_CATCH_ENV_BEGIN;
+  return env_val(sort_box(new Sort(mut_tm_unbox(tm)->getRegExpSort())),
+                 ioWorld);
+  CVC5_LEAN_API_TRY_CATCH_ENV_END(ioWorld);
+}
+
+LEAN_EXPORT lean_obj_res termManager_getRoundingModeSort(lean_obj_arg tm,
+                                                         lean_obj_arg ioWorld)
+{
+  CVC5_LEAN_API_TRY_CATCH_ENV_BEGIN;
+  return env_val(sort_box(new Sort(mut_tm_unbox(tm)->getRoundingModeSort())),
+                 ioWorld);
+  CVC5_LEAN_API_TRY_CATCH_ENV_END(ioWorld);
+}
+
+LEAN_EXPORT lean_obj_res termManager_getStringSort(lean_obj_arg tm,
+                                                   lean_obj_arg ioWorld)
+{
+  CVC5_LEAN_API_TRY_CATCH_ENV_BEGIN;
+  return env_val(sort_box(new Sort(mut_tm_unbox(tm)->getStringSort())),
+                 ioWorld);
+  CVC5_LEAN_API_TRY_CATCH_ENV_END(ioWorld);
+}
+
+LEAN_EXPORT lean_obj_res termManager_mkArraySort(lean_obj_arg tm,
+                                                 lean_obj_arg idxSort,
+                                                 lean_obj_arg elmSort,
+                                                 lean_obj_arg ioWorld)
+{
+  CVC5_LEAN_API_TRY_CATCH_ENV_BEGIN;
+  return env_val(sort_box(new Sort(mut_tm_unbox(tm)->mkArraySort(
+                     *sort_unbox(idxSort), *sort_unbox(elmSort)))),
+                 ioWorld);
+  CVC5_LEAN_API_TRY_CATCH_ENV_END(ioWorld);
+}
+
+LEAN_EXPORT lean_obj_res termManager_mkBitVectorSort(lean_obj_arg tm,
+                                                     uint32_t size,
+                                                     lean_obj_arg ioWorld)
+{
+  CVC5_LEAN_API_TRY_CATCH_ENV_BEGIN;
+  return env_val(sort_box(new Sort(mut_tm_unbox(tm)->mkBitVectorSort(size))),
+                 ioWorld);
+  CVC5_LEAN_API_TRY_CATCH_ENV_END(ioWorld);
+}
+
+LEAN_EXPORT lean_obj_res termManager_mkFloatingPointSort(lean_obj_arg tm,
+                                                         uint32_t exp,
+                                                         uint32_t sig,
+                                                         lean_obj_arg ioWorld)
+{
+  CVC5_LEAN_API_TRY_CATCH_ENV_BEGIN;
+  return env_val(
+      sort_box(new Sort(mut_tm_unbox(tm)->mkFloatingPointSort(exp, sig))),
+      ioWorld);
+  CVC5_LEAN_API_TRY_CATCH_ENV_END(ioWorld);
+}
+
+LEAN_EXPORT lean_obj_res termManager_mkFiniteFieldSortOfString(
+    lean_obj_arg tm, lean_obj_arg size, uint32_t base, lean_obj_arg ioWorld)
+{
+  CVC5_LEAN_API_TRY_CATCH_ENV_BEGIN;
+  return env_val(sort_box(new Sort(mut_tm_unbox(tm)->mkFiniteFieldSort(
+                     lean_string_cstr(size), base))),
+                 ioWorld);
+  CVC5_LEAN_API_TRY_CATCH_ENV_END(ioWorld);
+}
+
+LEAN_EXPORT lean_obj_res termManager_mkFunctionSort(lean_obj_arg tm,
+                                                    lean_obj_arg sorts,
+                                                    lean_obj_arg codomain,
+                                                    lean_obj_arg ioWorld)
+{
+  CVC5_LEAN_API_TRY_CATCH_ENV_BEGIN;
+  std::vector<Sort> cvc5Sorts;
+  for (size_t i = 0, n = lean_array_size(sorts); i < n; ++i)
+  {
+    cvc5Sorts.push_back(*sort_unbox(
+        lean_array_get(sort_box(new Sort()), sorts, lean_usize_to_nat(i))));
+  }
+  return env_val(sort_box(new Sort(mut_tm_unbox(tm)->mkFunctionSort(
+                     cvc5Sorts, *sort_unbox(codomain)))),
+                 ioWorld);
+  CVC5_LEAN_API_TRY_CATCH_ENV_END(ioWorld);
+}
+
+LEAN_EXPORT lean_obj_res termManager_mkPredicateSort(lean_obj_arg tm,
+                                                     lean_obj_arg sorts,
+                                                     lean_obj_arg ioWorld)
+{
+  CVC5_LEAN_API_TRY_CATCH_ENV_BEGIN;
+  std::vector<Sort> cvc5Sorts;
+  for (size_t i = 0, n = lean_array_size(sorts); i < n; ++i)
+  {
+    cvc5Sorts.push_back(*sort_unbox(
+        lean_array_get(sort_box(new Sort()), sorts, lean_usize_to_nat(i))));
+  }
+  return env_val(
+      sort_box(new Sort(mut_tm_unbox(tm)->mkPredicateSort(cvc5Sorts))),
+      ioWorld);
+  CVC5_LEAN_API_TRY_CATCH_ENV_END(ioWorld);
+}
+
+LEAN_EXPORT lean_obj_res termManager_mkTupleSort(lean_obj_arg tm,
+                                                 lean_obj_arg sorts,
+                                                 lean_obj_arg ioWorld)
+{
+  CVC5_LEAN_API_TRY_CATCH_ENV_BEGIN;
+  std::vector<Sort> cvc5Sorts;
+  for (size_t i = 0, n = lean_array_size(sorts); i < n; ++i)
+  {
+    cvc5Sorts.push_back(*sort_unbox(
+        lean_array_get(sort_box(new Sort()), sorts, lean_usize_to_nat(i))));
+  }
+  return env_val(sort_box(new Sort(mut_tm_unbox(tm)->mkTupleSort(cvc5Sorts))),
+                 ioWorld);
+  CVC5_LEAN_API_TRY_CATCH_ENV_END(ioWorld);
+}
+
+LEAN_EXPORT lean_obj_res termManager_mkSetSort(lean_obj_arg tm,
+                                               lean_obj_arg sort,
+                                               lean_obj_arg ioWorld)
+{
+  CVC5_LEAN_API_TRY_CATCH_ENV_BEGIN;
+  return env_val(
+      sort_box(new Sort(mut_tm_unbox(tm)->mkSetSort(*sort_unbox(sort)))),
+      ioWorld);
+  CVC5_LEAN_API_TRY_CATCH_ENV_END(ioWorld);
+}
+
+LEAN_EXPORT lean_obj_res termManager_mkBagSort(lean_obj_arg tm,
+                                               lean_obj_arg sort,
+                                               lean_obj_arg ioWorld)
+{
+  CVC5_LEAN_API_TRY_CATCH_ENV_BEGIN;
+  return env_val(
+      sort_box(new Sort(mut_tm_unbox(tm)->mkBagSort(*sort_unbox(sort)))),
+      ioWorld);
+  CVC5_LEAN_API_TRY_CATCH_ENV_END(ioWorld);
+}
+
+LEAN_EXPORT lean_obj_res termManager_mkSequenceSort(lean_obj_arg tm,
+                                                    lean_obj_arg sort,
+                                                    lean_obj_arg ioWorld)
+{
+  CVC5_LEAN_API_TRY_CATCH_ENV_BEGIN;
+  return env_val(
+      sort_box(new Sort(mut_tm_unbox(tm)->mkSequenceSort(*sort_unbox(sort)))),
+      ioWorld);
+  CVC5_LEAN_API_TRY_CATCH_ENV_END(ioWorld);
+}
+
+LEAN_EXPORT lean_obj_res termManager_mkAbstractSort(lean_obj_arg tm,
+                                                    uint16_t kind,
+                                                    lean_obj_arg ioWorld)
+{
+  CVC5_LEAN_API_TRY_CATCH_ENV_BEGIN;
+  SortKind k = static_cast<SortKind>(static_cast<int32_t>(kind) - 2);
+  return env_val(sort_box(new Sort(mut_tm_unbox(tm)->mkAbstractSort(k))),
+                 ioWorld);
+  CVC5_LEAN_API_TRY_CATCH_ENV_END(ioWorld);
+}
+
+LEAN_EXPORT lean_obj_res termManager_mkUninterpretedSort(lean_obj_arg tm,
+                                                         lean_obj_arg symbol,
+                                                         lean_obj_arg ioWorld)
+{
+  CVC5_LEAN_API_TRY_CATCH_ENV_BEGIN;
+  return env_val(sort_box(new Sort(mut_tm_unbox(tm)->mkUninterpretedSort(
+                     lean_string_cstr(symbol)))),
+                 ioWorld);
+  CVC5_LEAN_API_TRY_CATCH_ENV_END(ioWorld);
+}
+
+LEAN_EXPORT lean_obj_arg
+termManager_mkUninterpretedSortConstructorSort(lean_obj_arg tm,
+                                               lean_obj_arg arity,
+                                               lean_obj_arg symbol,
+                                               lean_obj_arg ioWorld)
+{
+  CVC5_LEAN_API_TRY_CATCH_ENV_BEGIN;
+  return env_val(
+      sort_box(new Sort(mut_tm_unbox(tm)->mkUninterpretedSortConstructorSort(
+          lean_usize_of_nat(arity), lean_string_cstr(symbol)))),
+      ioWorld);
+  CVC5_LEAN_API_TRY_CATCH_ENV_END(ioWorld);
+}
+
+LEAN_EXPORT lean_obj_res termManager_mkNullableSort(lean_obj_arg tm,
+                                                    lean_obj_arg sort,
+                                                    lean_obj_arg ioWorld)
+{
+  CVC5_LEAN_API_TRY_CATCH_ENV_BEGIN;
+  return env_val(
+      sort_box(new Sort(mut_tm_unbox(tm)->mkNullableSort(*sort_unbox(sort)))),
+      ioWorld);
+  CVC5_LEAN_API_TRY_CATCH_ENV_END(ioWorld);
+}
+
+LEAN_EXPORT lean_obj_res termManager_mkParamSort(lean_obj_arg tm,
+                                                 lean_obj_arg symbol,
+                                                 lean_obj_arg ioWorld)
+{
+  CVC5_LEAN_API_TRY_CATCH_ENV_BEGIN;
+  return env_val(sort_box(new Sort(
+                     mut_tm_unbox(tm)->mkParamSort(lean_string_cstr(symbol)))),
+                 ioWorld);
+  CVC5_LEAN_API_TRY_CATCH_ENV_END(ioWorld);
+}
+
+// # Terms
+
+LEAN_EXPORT lean_obj_res termManager_mkBoolean(lean_obj_arg tm,
+                                               uint8_t val,
+                                               lean_obj_arg ioWorld)
+{
+  CVC5_LEAN_API_TRY_CATCH_ENV_BEGIN;
+  return env_val(
+      term_box(new Term(mut_tm_unbox(tm)->mkBoolean(bool_unbox(val)))),
+      ioWorld);
+  CVC5_LEAN_API_TRY_CATCH_ENV_END(ioWorld);
+}
+
+LEAN_EXPORT lean_obj_res termManager_mkIntegerFromString(lean_obj_arg tm,
+                                                         lean_obj_arg val,
+                                                         lean_obj_arg ioWorld)
+{
+  CVC5_LEAN_API_TRY_CATCH_ENV_BEGIN;
+  return env_val(
+      term_box(new Term(mut_tm_unbox(tm)->mkInteger(lean_string_cstr(val)))),
+      ioWorld);
+  CVC5_LEAN_API_TRY_CATCH_ENV_END(ioWorld);
+}
+
+LEAN_EXPORT lean_obj_res termManager_mkRealFromString(lean_obj_arg tm,
+                                                      lean_obj_arg val,
+                                                      lean_obj_arg ioWorld)
+{
+  CVC5_LEAN_API_TRY_CATCH_ENV_BEGIN;
+  return env_val(
+      term_box(new Term(mut_tm_unbox(tm)->mkReal(lean_string_cstr(val)))),
+      ioWorld);
+  CVC5_LEAN_API_TRY_CATCH_ENV_END(ioWorld);
+}
+
+LEAN_EXPORT lean_obj_res termManager_mkTerm(lean_obj_arg tm,
+                                            uint16_t kind,
+                                            lean_obj_arg children,
+                                            lean_obj_arg ioWorld)
+{
+  CVC5_LEAN_API_TRY_CATCH_ENV_BEGIN;
+  Kind k = static_cast<Kind>(static_cast<int32_t>(kind) - 2);
+  std::vector<Term> cs;
+  for (size_t i = 0, n = lean_array_size(children); i < n; ++i)
+  {
+    cs.push_back(*term_unbox(
+        lean_array_get(term_box(new Term()), children, lean_usize_to_nat(i))));
+  }
+  return env_val(term_box(new Term(mut_tm_unbox(tm)->mkTerm(k, cs))), ioWorld);
+  CVC5_LEAN_API_TRY_CATCH_ENV_END(ioWorld);
+}
+
+LEAN_EXPORT lean_obj_res termManager_mkTermOfOp(lean_obj_arg tm,
+                                                lean_obj_arg op,
+                                                lean_obj_arg children,
+                                                lean_obj_arg ioWorld)
+{
+  CVC5_LEAN_API_TRY_CATCH_ENV_BEGIN;
+  std::vector<Term> cs;
+  for (size_t i = 0, n = lean_array_size(children); i < n; ++i)
+  {
+    cs.push_back(*term_unbox(
+        lean_array_get(term_box(new Term()), children, lean_usize_to_nat(i))));
+  }
+  return env_val(
+      term_box(new Term(mut_tm_unbox(tm)->mkTerm(*op_unbox(op), cs))), ioWorld);
+  CVC5_LEAN_API_TRY_CATCH_ENV_END(ioWorld);
+}
+
+LEAN_EXPORT lean_obj_res termManager_mkConst(lean_obj_arg tm,
+                                             lean_obj_arg sort,
+                                             lean_obj_arg symbol,
+                                             lean_obj_arg ioWorld)
+{
+  CVC5_LEAN_API_TRY_CATCH_ENV_BEGIN;
+  return env_val(term_box(new Term(mut_tm_unbox(tm)->mkConst(
+                     *sort_unbox(sort), lean_string_cstr(symbol)))),
+                 ioWorld);
+  CVC5_LEAN_API_TRY_CATCH_ENV_END(ioWorld);
+}
+
+LEAN_EXPORT lean_obj_res termManager_mkVar(lean_obj_arg tm,
+                                           lean_obj_arg sort,
+                                           lean_obj_arg symbol,
+                                           lean_obj_arg ioWorld)
+{
+  CVC5_LEAN_API_TRY_CATCH_ENV_BEGIN;
+  return env_val(term_box(new Term(mut_tm_unbox(tm)->mkVar(
+                     *sort_unbox(sort), lean_string_cstr(symbol)))),
+                 ioWorld);
+  CVC5_LEAN_API_TRY_CATCH_ENV_END(ioWorld);
+}
+
+LEAN_EXPORT lean_obj_res termManager_mkOpOfIndices(lean_obj_arg tm,
+                                                   uint16_t kind,
+                                                   lean_obj_arg args,
+                                                   lean_obj_arg ioWorld)
+{
+  CVC5_LEAN_API_TRY_CATCH_ENV_BEGIN;
+  Kind k = static_cast<Kind>(static_cast<int32_t>(kind) - 2);
+  std::vector<uint32_t> indices;
+  for (size_t i = 0, n = lean_array_size(args); i < n; ++i)
+  {
+    indices.push_back(lean_uint32_of_nat_mk(
+        lean_array_get(lean_usize_to_nat(0), args, lean_usize_to_nat(i))));
+  }
+  return env_val(op_box(new Op(mut_tm_unbox(tm)->mkOp(k, indices))), ioWorld);
+  CVC5_LEAN_API_TRY_CATCH_ENV_END(ioWorld);
+}
+
+// ### Solver imports/helpers
+
+LEAN_EXPORT lean_obj_res env_newSolver(lean_obj_arg tm, lean_obj_arg ioWorld)
+{
+  CVC5_LEAN_API_TRY_CATCH_ENV_BEGIN;
+  return env_val(solver_box(new Solver(*mut_tm_unbox(tm))), ioWorld);
+  CVC5_LEAN_API_TRY_CATCH_ENV_END(ioWorld);
+}
+
+// Retrieves the lean-obj for the "raw" (C++) solver.
+b_lean_obj_res ffi_solver_to_raw(b_lean_obj_arg safe_solver);
+
+// Builds on `ffi_lover_to_raw` to return the lean-unboxed "raw" (C++) solver.
+static inline Solver* extract_solver(b_lean_obj_arg safe_solver)
+{
+  return static_cast<Solver*>(
+      lean_get_external_data(ffi_solver_to_raw(safe_solver)));
+}
+
+LEAN_EXPORT lean_obj_res solver_getVersion(b_lean_obj_arg solver,
+                                           lean_obj_arg ioWorld)
+{
+  CVC5_LEAN_API_TRY_CATCH_ENV_BEGIN;
+  return env_val(lean_mk_string(extract_solver(solver)->getVersion().c_str()),
+                 ioWorld);
+  CVC5_LEAN_API_TRY_CATCH_ENV_END(ioWorld);
+}
+
+LEAN_EXPORT lean_obj_res solver_setOption(lean_obj_arg solver,
                                           lean_object* option,
                                           lean_object* value,
-                                          lean_obj_arg solver)
+                                          lean_obj_arg ioWorld)
 {
-  CVC5_LEAN_API_TRY_CATCH_SOLVER_BEGIN;
-  solver_unbox(solver)->setOption(lean_string_cstr(option),
-                                  lean_string_cstr(value));
-  return solver_val(lean_box(0), inst, lean_box(0), mk_unit_unit(), solver);
-  CVC5_LEAN_API_TRY_CATCH_SOLVER_END(inst, solver);
+  CVC5_LEAN_API_TRY_CATCH_ENV_BEGIN;
+  extract_solver(solver)->setOption(lean_string_cstr(option),
+                                    lean_string_cstr(value));
+  return env_val(mk_unit_unit(), ioWorld);
+  CVC5_LEAN_API_TRY_CATCH_ENV_END(ioWorld);
 }
 
-LEAN_EXPORT lean_obj_res solver_resetAssertions(lean_obj_arg inst,
-                                                lean_obj_arg solver)
+LEAN_EXPORT lean_obj_res solver_resetAssertions(lean_obj_arg solver,
+
+                                                lean_obj_arg ioWorld)
 {
-  CVC5_LEAN_API_TRY_CATCH_SOLVER_BEGIN;
-  solver_unbox(solver)->resetAssertions();
-  return solver_val(lean_box(0), inst, lean_box(0), mk_unit_unit(), solver);
-  CVC5_LEAN_API_TRY_CATCH_SOLVER_END(inst, solver);
+  CVC5_LEAN_API_TRY_CATCH_ENV_BEGIN;
+  extract_solver(solver)->resetAssertions();
+  return env_val(mk_unit_unit(), ioWorld);
+  CVC5_LEAN_API_TRY_CATCH_ENV_END(ioWorld);
 }
 
-LEAN_EXPORT lean_obj_res solver_setLogic(lean_obj_arg inst,
+LEAN_EXPORT lean_obj_res solver_setLogic(lean_obj_arg solver,
                                          lean_object* logic,
-                                         lean_obj_arg solver)
+
+                                         lean_obj_arg ioWorld)
 {
-  CVC5_LEAN_API_TRY_CATCH_SOLVER_BEGIN;
-  solver_unbox(solver)->setLogic(lean_string_cstr(logic));
-  return solver_val(lean_box(0), inst, lean_box(0), mk_unit_unit(), solver);
-  CVC5_LEAN_API_TRY_CATCH_SOLVER_END(inst, solver);
+  CVC5_LEAN_API_TRY_CATCH_ENV_BEGIN;
+  extract_solver(solver)->setLogic(lean_string_cstr(logic));
+  return env_val(mk_unit_unit(), ioWorld);
+  CVC5_LEAN_API_TRY_CATCH_ENV_END(ioWorld);
 }
 
-LEAN_EXPORT lean_obj_res solver_simplify(lean_obj_arg inst,
+LEAN_EXPORT lean_obj_res solver_simplify(lean_obj_arg solver,
                                          lean_obj_arg term,
                                          lean_obj_arg applySubs,
-                                         lean_obj_arg solver)
+
+                                         lean_obj_arg ioWorld)
 {
-  CVC5_LEAN_API_TRY_CATCH_SOLVER_BEGIN;
-  Term value = solver_unbox(solver)->simplify(
+  CVC5_LEAN_API_TRY_CATCH_ENV_BEGIN;
+  Term value = extract_solver(solver)->simplify(
       *term_unbox(term), bool_unbox(lean_unbox(applySubs)));
-  return solver_val(
-      lean_box(0), inst, lean_box(0), term_box(new Term(value)), solver);
-  CVC5_LEAN_API_TRY_CATCH_SOLVER_END(inst, solver);
+  return env_val(term_box(new Term(value)), ioWorld);
+  CVC5_LEAN_API_TRY_CATCH_ENV_END(ioWorld);
 }
 
-LEAN_EXPORT lean_obj_res solver_declareFun(lean_obj_arg inst,
+LEAN_EXPORT lean_obj_res solver_declareFun(lean_obj_arg solver,
                                            lean_obj_arg symbol,
                                            lean_obj_arg sorts,
                                            lean_obj_arg sort,
                                            uint8_t fresh,
-                                           lean_obj_arg solver)
+
+                                           lean_obj_arg ioWorld)
 {
-  CVC5_LEAN_API_TRY_CATCH_SOLVER_BEGIN;
+  CVC5_LEAN_API_TRY_CATCH_ENV_BEGIN;
   std::vector<Sort> ss;
   for (size_t i = 0, n = lean_array_size(sorts); i < n; ++i)
   {
     ss.push_back(*sort_unbox(
         lean_array_get(sort_box(new Sort()), sorts, lean_usize_to_nat(i))));
   }
-  Term f = solver_unbox(solver)->declareFun(
+  Term f = extract_solver(solver)->declareFun(
       lean_string_cstr(symbol), ss, *sort_unbox(sort), bool_unbox(fresh));
-  return solver_val(
-      lean_box(0), inst, lean_box(0), term_box(new Term(f)), solver);
-  CVC5_LEAN_API_TRY_CATCH_SOLVER_END(inst, solver);
+  return env_val(term_box(new Term(f)), ioWorld);
+  CVC5_LEAN_API_TRY_CATCH_ENV_END(ioWorld);
 }
 
-LEAN_EXPORT lean_obj_res solver_assertFormula(lean_obj_arg inst,
+LEAN_EXPORT lean_obj_res solver_assertFormula(lean_obj_arg solver,
                                               lean_object* term,
-                                              lean_obj_arg solver)
+
+                                              lean_obj_arg ioWorld)
 {
-  CVC5_LEAN_API_TRY_CATCH_SOLVER_BEGIN;
-  solver_unbox(solver)->assertFormula(*term_unbox(term));
-  return solver_val(lean_box(0), inst, lean_box(0), mk_unit_unit(), solver);
-  CVC5_LEAN_API_TRY_CATCH_SOLVER_END(inst, solver);
+  CVC5_LEAN_API_TRY_CATCH_ENV_BEGIN;
+  extract_solver(solver)->assertFormula(*term_unbox(term));
+  return env_val(mk_unit_unit(), ioWorld);
+  CVC5_LEAN_API_TRY_CATCH_ENV_END(ioWorld);
 }
 
-LEAN_EXPORT lean_obj_res solver_checkSat(lean_obj_arg inst, lean_obj_arg solver)
+LEAN_EXPORT lean_obj_res solver_checkSat(lean_obj_arg solver,
+                                         lean_obj_arg ioWorld)
 {
-  CVC5_LEAN_API_TRY_CATCH_SOLVER_BEGIN;
-  return solver_val(lean_box(0),
-                    inst,
-                    lean_box(0),
-                    result_box(new Result(solver_unbox(solver)->checkSat())),
-                    solver);
-  CVC5_LEAN_API_TRY_CATCH_SOLVER_END(inst, solver);
+  CVC5_LEAN_API_TRY_CATCH_ENV_BEGIN;
+  return env_val(result_box(new Result(extract_solver(solver)->checkSat())),
+                 ioWorld);
+  CVC5_LEAN_API_TRY_CATCH_ENV_END(ioWorld);
 }
 
-LEAN_EXPORT lean_obj_res solver_checkSatAssuming(lean_obj_arg inst,
+LEAN_EXPORT lean_obj_res solver_checkSatAssuming(lean_obj_arg solver,
                                                  lean_obj_arg assumptions,
-                                                 lean_obj_arg solver)
+
+                                                 lean_obj_arg ioWorld)
 {
-  CVC5_LEAN_API_TRY_CATCH_SOLVER_BEGIN;
+  CVC5_LEAN_API_TRY_CATCH_ENV_BEGIN;
   std::vector<Term> formulas;
   for (size_t i = 0, n = lean_array_size(assumptions); i < n; ++i)
   {
     formulas.push_back(*term_unbox(lean_array_get(
         term_box(new Term()), assumptions, lean_usize_to_nat(i))));
   }
-  Result res = solver_unbox(solver)->checkSatAssuming(formulas);
-  return solver_val(
-      lean_box(0), inst, lean_box(0), result_box(new Result(res)), solver);
-  CVC5_LEAN_API_TRY_CATCH_SOLVER_END(inst, solver);
+  Result res = extract_solver(solver)->checkSatAssuming(formulas);
+  return env_val(result_box(new Result(res)), ioWorld);
+  CVC5_LEAN_API_TRY_CATCH_ENV_END(ioWorld);
 }
 
-LEAN_EXPORT lean_obj_res solver_getUnsatCore(lean_obj_arg inst,
-                                             lean_obj_arg solver)
+LEAN_EXPORT lean_obj_res solver_getUnsatCore(lean_obj_arg solver,
+                                             lean_obj_arg ioWorld)
 {
-  CVC5_LEAN_API_TRY_CATCH_SOLVER_BEGIN;
+  CVC5_LEAN_API_TRY_CATCH_ENV_BEGIN;
   std::vector<Term> assertions = solver_unbox(solver)->getUnsatCore();
   lean_object* as = lean_mk_empty_array();
   for (const Term& assertion : assertions)
   {
     as = lean_array_push(as, term_box(new Term(assertion)));
   }
-  return solver_val(lean_box(0), inst, lean_box(0), as, solver);
-  CVC5_LEAN_API_TRY_CATCH_SOLVER_END(inst, solver);
+  return env_val(as, ioWorld);
+  CVC5_LEAN_API_TRY_CATCH_ENV_END(ioWorld);
 }
 
-LEAN_EXPORT lean_obj_res solver_getProof(lean_obj_arg inst, lean_obj_arg solver)
+LEAN_EXPORT lean_obj_res solver_getProof(lean_obj_arg solver,
+
+                                         lean_obj_arg ioWorld)
 {
-  CVC5_LEAN_API_TRY_CATCH_SOLVER_BEGIN;
-  std::vector<Proof> proofs = solver_unbox(solver)->getProof();
+  CVC5_LEAN_API_TRY_CATCH_ENV_BEGIN;
+  std::vector<Proof> proofs = extract_solver(solver)->getProof();
   lean_object* ps = lean_mk_empty_array();
   for (const Proof& proof : proofs)
   {
     ps = lean_array_push(ps, proof_box(new Proof(proof)));
   }
-  return solver_val(lean_box(0), inst, lean_box(0), ps, solver);
-  CVC5_LEAN_API_TRY_CATCH_SOLVER_END(inst, solver);
+  return env_val(ps, ioWorld);
+  CVC5_LEAN_API_TRY_CATCH_ENV_END(ioWorld);
 }
 
-LEAN_EXPORT lean_obj_res solver_getValue(lean_obj_arg inst,
+LEAN_EXPORT lean_obj_res solver_getValue(lean_obj_arg solver,
                                          lean_obj_arg term,
-                                         lean_obj_arg solver)
+
+                                         lean_obj_arg ioWorld)
 {
-  CVC5_LEAN_API_TRY_CATCH_SOLVER_BEGIN;
-  return solver_val(
-      lean_box(0),
-      inst,
-      lean_box(0),
-      term_box(new Term(solver_unbox(solver)->getValue(*term_unbox(term)))),
-      solver);
-  CVC5_LEAN_API_TRY_CATCH_SOLVER_END(inst, solver);
+  CVC5_LEAN_API_TRY_CATCH_ENV_BEGIN;
+  return env_val(
+      term_box(new Term(extract_solver(solver)->getValue(*term_unbox(term)))),
+      ioWorld);
+  CVC5_LEAN_API_TRY_CATCH_ENV_END(ioWorld);
 }
 
-LEAN_EXPORT lean_obj_res solver_getValues(lean_obj_arg inst,
+LEAN_EXPORT lean_obj_res solver_getValues(lean_obj_arg solver,
                                           lean_obj_arg terms,
-                                          lean_obj_arg solver)
+
+                                          lean_obj_arg ioWorld)
 {
-  CVC5_LEAN_API_TRY_CATCH_SOLVER_BEGIN;
+  CVC5_LEAN_API_TRY_CATCH_ENV_BEGIN;
   std::vector<Term> ts;
   for (size_t i = 0, n = lean_array_size(terms); i < n; ++i)
   {
     ts.push_back(*term_unbox(
         lean_array_get(term_box(new Term()), terms, lean_usize_to_nat(i))));
   }
-  std::vector<Term> values = solver_unbox(solver)->getValue(ts);
+  std::vector<Term> values = extract_solver(solver)->getValue(ts);
   lean_object* vs = lean_mk_empty_array();
   for (const Term& value : values)
   {
     vs = lean_array_push(vs, term_box(new Term(value)));
   }
-  return solver_val(lean_box(0), inst, lean_box(0), vs, solver);
-  CVC5_LEAN_API_TRY_CATCH_SOLVER_END(inst, solver);
+  return env_val(vs, ioWorld);
+  CVC5_LEAN_API_TRY_CATCH_ENV_END(ioWorld);
 }
 
-LEAN_EXPORT lean_obj_res solver_getModelDomainElements(lean_obj_arg inst,
+LEAN_EXPORT lean_obj_res solver_getModelDomainElements(lean_obj_arg solver,
                                                        lean_obj_arg sort,
-                                                       lean_obj_arg solver)
+                                                       lean_obj_arg ioWorld)
 {
-  CVC5_LEAN_API_TRY_CATCH_SOLVER_BEGIN;
-  std::vector<Term> elements = solver_unbox(solver)->getModelDomainElements(*sort_unbox(sort));
+  CVC5_LEAN_API_TRY_CATCH_ENV_BEGIN;
+  std::vector<Term> elements =
+      solver_unbox(solver)->getModelDomainElements(*sort_unbox(sort));
   lean_object* es = lean_mk_empty_array();
   for (const Term& element : elements)
   {
     es = lean_array_push(es, term_box(new Term(element)));
   }
-  return solver_val(lean_box(0), inst, lean_box(0), es, solver);
-  CVC5_LEAN_API_TRY_CATCH_SOLVER_END(inst, solver);
+  return env_val(es, ioWorld);
+  CVC5_LEAN_API_TRY_CATCH_ENV_END(ioWorld);
 }
 
-LEAN_EXPORT lean_obj_res solver_proofToString(lean_obj_arg inst,
+LEAN_EXPORT lean_obj_res solver_proofToString(lean_obj_arg solver,
                                               lean_obj_arg proof,
-                                              lean_obj_arg solver)
+
+                                              lean_obj_arg ioWorld)
 {
-  CVC5_LEAN_API_TRY_CATCH_SOLVER_BEGIN;
-  return solver_val(
-      lean_box(0),
-      inst,
-      lean_box(0),
+  CVC5_LEAN_API_TRY_CATCH_ENV_BEGIN;
+  return env_val(
       lean_mk_string(
-          solver_unbox(solver)->proofToString(*proof_unbox(proof)).c_str()),
-      solver);
-  CVC5_LEAN_API_TRY_CATCH_SOLVER_END(inst, solver);
+          extract_solver(solver)->proofToString(*proof_unbox(proof)).c_str()),
+      ioWorld);
+  CVC5_LEAN_API_TRY_CATCH_ENV_END(ioWorld);
 }
 
-LEAN_EXPORT lean_obj_res solver_parseCommands(lean_obj_arg inst,
+LEAN_EXPORT lean_obj_res solver_parseCommands(lean_obj_arg solver,
                                               lean_obj_arg query,
-                                              lean_obj_arg solver)
+
+                                              lean_obj_arg ioWorld)
 {
-  CVC5_LEAN_API_TRY_CATCH_SOLVER_BEGIN;
-  Solver* slv = solver_unbox(solver);
+  CVC5_LEAN_API_TRY_CATCH_ENV_BEGIN;
+  Solver* slv = extract_solver(solver);
   // construct an input parser associated the solver above
   parser::InputParser parser(slv);
   // get the symbol manager of the parser, used when invoking commands below
@@ -1700,23 +1748,7 @@ LEAN_EXPORT lean_obj_res solver_parseCommands(lean_obj_arg inst,
     // to out
     cmd.invoke(slv, sm, out);
   }
-  std::vector<Sort> sortVars = sm->getDeclaredSorts();
-  lean_object* svs = lean_mk_empty_array();
-  for (const Sort& sortVar : sortVars)
-  {
-    svs = lean_array_push(svs, sort_box(new Sort(sortVar)));
-  }
-  std::vector<Term> termVars = sm->getDeclaredTerms();
-  lean_object* tvs = lean_mk_empty_array();
-  for (const Term& termVar : termVars)
-  {
-    tvs = lean_array_push(tvs, term_box(new Term(termVar)));
-  }
-  return solver_val(lean_box(0),
-                    inst,
-                    lean_box(0),
-                    prod_mk(lean_box(0), lean_box(0), svs, tvs),
-                    solver);
-  CVC5_LEAN_API_TRY_CATCH_SOLVER_END(inst, solver);
+  return env_val(mk_unit_unit(), ioWorld);
+  CVC5_LEAN_API_TRY_CATCH_ENV_END(ioWorld);
 }
 }
