cvc5Test/Unit/ApiSkolemId.lean
@@ -7,13 +7,13 @@ import cvc5Test.Init
 
 namespace cvc5.Test
 
-test![TestApiBlackSkolemId, skolemIdToString] _tm => do
+test![TestApiBlackSkolemId, skolemIdToString] do
   for idx in [SkolemId.INTERNAL.toCtorIdx : SkolemId.NONE.toCtorIdx] do
     let si := SkolemId.ofNat idx
     -- if this assertion fails, the switch in `enum_to_string.cpp` is missing id `si`.
     assertNe si.toString "?"
 
-test![TestApiBlackSkolemId, skolemIdHash] _tm => do
+test![TestApiBlackSkolemId, skolemIdHash] do
   for idx in [SkolemId.INTERNAL.toCtorIdx : SkolemId.NONE.toCtorIdx] do
     let si := SkolemId.ofNat idx
     assertEq si.hash ⟨si.toCtorIdx⟩
